add some graph operations, state transitivity lemma.

src/GraphInterface.v
@@ -26,5 +26,47 @@ Class ok {vertex} {graph : graph vertex} : Prop := {
     edges_NoDup : forall g u, NoDup (edges g u);
   }.
 Arguments ok {_} _.
+
+Section ops.
+  Context {vertex : Type} {graph : graph vertex} {ok : ok graph}.
+
+  Definition put_edges g u vs :=
+    fold_left (fun g v => put g u v) vs g.
+
+  Definition union g1 g2 :=
+    fold_left (fun g u => put_edges g u (edges g2 u)) (sources g2) g1.
+
+  Lemma edges_put_edges g u vs u' v' :
+    In v' (edges (put_edges g u vs) u') <->
+      In v' (edges g u') \/ u = u' /\ In v' vs.
+  Proof.
+    unfold put_edges. revert g. induction vs as [|a vs IH]; intros g; cbn [fold_left].
+    - cbn [In]. tauto.
+    - rewrite IH, edges_put. cbn [In]. tauto.
+  Qed.
+
+  Lemma edges_fold_union ss g1 g2 u' v' :
+    In v' (edges (fold_left (fun g u => put_edges g u (edges g2 u)) ss g1) u') <->
+      In v' (edges g1 u') \/ In u' ss /\ In v' (edges g2 u').
+  Proof.
+    revert g1. induction ss as [|a ss IH]; intros g1; cbn [fold_left In].
+    - tauto.
+    - rewrite IH, edges_put_edges. cbn [In].
+      split.
+      + intros [[?|[-> ?]]|[? ?]]; auto 7.
+      + intros [?|[[->|?] ?]]; auto 7.
+  Qed.
+
+  Lemma edges_union g1 g2 u' v' :
+    In v' (edges (union g1 g2) u') <->
+      In v' (edges g1 u') \/ In v' (edges g2 u').
+  Proof.
+    unfold union. rewrite edges_fold_union.
+    split.
+    - intros [H|[_ H]]; auto.
+    - intros [H|H]; [auto|]. right. split; [|exact H].
+      apply (proj2 (sources_spec g2 u')). intro Hnil. rewrite Hnil in H. exact H.
+  Qed.
+End ops.
 End graph.
 Global Coercion graph.rep : graph.graph >-> Sortclass.
